Classes/Monad.v
@@ -22,16 +22,16 @@ Hint Unfold bindM : soundness.
 Hint Rewrite @bind_id_left @bind_id_right @bind_assoc : soundness.
 
 Class bind_sound (M M' : Type → Type) {MM : Monad M} {MM' : Monad M'} 
-  {GM : ∀ A A', Galois A A' → Galois (M A) (M' A')} := 
-  bindM_sound : ∀ {A A' B B'} {GA : Galois A A'} {GB : Galois B B'} 
+  {GM : ∀ A A', Galois A A' → Galois (M A) (M' A')} : Prop := 
+  bindM_sound : ∀ {A A' B B' : Type} {GA : Galois A A'} {GB : Galois B B'} 
     (m : M A) (m' : M' A') (f : A → M B) (f' : A' → M' B'),
     γ m m' → γ f f' → γ (bindM m f) (bindM m' f').
 
-Class return_sound (M M' : Type → Type) `{Monad M, Monad M'}
-  {GM : ∀ A A', Galois A A' → Galois (M A) (M' A')}
-  := 
-  returnM_sound : ∀ {A A'} {GA : Galois A A'} a a',
-    γ a a' → γ (returnM (M:=M) a) (returnM (M:=M') a').
+Class return_sound (M M' : Type → Type) {MM : Monad M} {MM' : Monad M'}
+  {GM : ∀ A A', Galois A A' → Galois (M A) (M' A')} : Prop :=
+  returnM_sound : ∀ {A A' : Type} {GA : Galois A A'} (a : A) (a' : A'),
+    γ (Galois:=GA) a a' → 
+    γ (Galois:=GM _ _ _) (returnM (M:=M) a) (returnM (M:=M') a').
 
 Definition join {M} `{Monad M} {A} 
   (mma : M (M A)) : M A :=
@@ -52,11 +52,11 @@ Notation "x ;; z" := (bindM x (λ _, z))
 
 Section MonadTransformer.
 
-  Class MonadT T `{TM_monad : ∀ (M : Type → Type) `{Monad M}, Monad (T M)} : Type :=
+  Class MonadT T {TM : ∀ (M : Type → Type) {MM : Monad M}, Monad (T M)} : Type :=
   {
-    liftT {M} `{Monad M} {A} : M A → T M A;
-    lift_return {M} `{Monad M} {A} : ∀ (x : A), liftT (returnM x) = returnM x;
-    lift_bind {M} `{Monad M} {A B} : ∀ (x : M A) (f : A → M B),
+    liftT {M} {MM : Monad M} {A} : M A → T M A;
+    lift_return {M} {MM : Monad M} {A} : ∀ (x : A), liftT (returnM x) = returnM x;
+    lift_bind {M} {MM : Monad M} {A B} : ∀ (x : M A) (f : A → M B),
       liftT (x >>= f) = liftT x >>= (f ∘ liftT);
   }.
 End MonadTransformer.
