Classes/Monad/MonadFail.v
@@ -1,8 +1,8 @@
 Require Export Base.
 Require Import Classes.Monad.
 
-Class MonadFail M `{M_monad : Monad M} : Type := {
-  fail {A : Type} : M A;
+Class MonadFail M {MM : Monad M} : Type := {
+  fail : ∀ {A : Type}, M A;
   fail_left: ∀ {A B} (m : A → M B), (@fail A) >>= m = fail;
 }.
 Arguments fail : simpl never.
