Classes/Monad/MonadState.v
@@ -1,8 +1,19 @@
 Require Export Base Coq.Strings.String.
 Require Import Classes.Monad.
+Require Import Classes.Galois.
 
-Class MonadState (S : Type) (M : Type -> Type) `{M_monad : Monad M} :=
+Class MonadState (S : Type) (M : Type -> Type) {MM : Monad M} :=
 {
   get : M S;
   put : S -> M unit;
 }.
+
+Class get_state_sound (M M' : Type → Type) {MM : Monad M} {MM' : Monad M'}
+  {GM : ∀ A A' : Type, Galois A A' → Galois (M A) (M' A')}
+  {S S' : Type} {GS : Galois S S'}  {MS : MonadState S M}
+  {MS' : MonadState S' M'} : Prop := get_sound : γ get get.
+
+Class put_state_sound (M M' : Type → Type) {MM : Monad M} {MM' : Monad M'}
+  {GM : ∀ A A' : Type, Galois A A' → Galois (M A) (M' A')}
+  {S S' : Type} {GS : Galois S S'}  {MS : MonadState S M}
+  {MS' : MonadState S' M'} : Prop := put_sound : ∀ s s', γ s s' → γ (put s) (put s').
