Types/Subtype.v
@@ -1,0 +1,73 @@
+Require Export Base.
+Require Import Classes.Galois.
+
+Class SubType (sub : Type) (super : Type) : Type := {
+  inject : sub → super;
+  project : super → option sub
+}.
+
+Class SubType_sound (super super' : Type) `{GS : Galois super super'} : Type :=
+{
+  inject_sound : ∀ {sub sub' : Type} {ST : SubType sub super}
+    {ST' : SubType sub' super'} {GS : Galois sub sub'} (s : sub) (s' : sub'),
+    γ s s' → γ (inject s) (inject s'); 
+  project_sound : ∀ {sub sub' : Type} {ST : SubType sub super}
+    {ST' : SubType sub' super'} {GS : Galois sub sub'} (s : super) (s' : super'),
+    γ s s' → γ (project s) (project s');
+}.
+
+Instance subtype_l : ∀ {A B}, SubType A (A + B) := {
+  inject := inl;
+  project := λ s, match s with | inl x => Some x | _ => None end
+}.
+
+Instance subtype_r : ∀ {A B}, SubType B (A+B) := {
+  inject := inr;
+  project := λ s, match s with | inr x => Some x | _ => None end
+}.
+
+Instance subtype_trans_r : ∀ {A B C} `{SubType A B}, SubType A (C + B) := {
+  inject := inject ∘ inr;
+  project := λ s, match s with | inr x => project x | _ => None end
+}.
+
+Instance subtype_trans_l {A B C} `{S : SubType A B} : SubType A (B + C).
+Proof. destruct S as [inject project]. split.
+  - exact (λ a, inl (inject a)).
+  - exact (λ bc, match bc with
+                 | inr _ => None
+                 | inl b => project b
+                 end).
+Defined.
+
+Instance subtype_top_r : ∀ A, SubType A (A+⊤) := {
+  inject := NotTop;
+  project := λ a, match a with
+                  | Top => None
+                  | NotTop x => Some x
+                  end;
+}.
+
+Instance subtype_bot_r : ∀ A, SubType A (A+⊥) := {
+  inject := NotBot;
+  project := λ a, match a with
+                  | Bot => None
+                  | NotBot x => Some x
+                  end;
+}.
+
+Instance subtype_top_l {A B} `{SubType A B} : 
+  SubType (A+⊤) (B+⊤).
+Proof. destruct H as [inject project]. split.
+  exact (λ a : (A+⊤), match a with
+                      | Top => Top
+                      | NotTop x => NotTop( inject x)
+                      end).
+  exact (λ b : (B+⊤), match b with
+                      | Top => None
+                      | NotTop x => match (project x) with
+                                    | Some x' => Some (NotTop x')
+                                    | None => None
+                                    end
+                      end).
+Defined.
